RegisterCounter.v
@@ -114,6 +114,160 @@ Proof.
     destruct ret; eauto. simpl. apply notin_union; eauto.
 Qed.
 
+(* Lemma final_preserves_binds_DInc5: forall st st' pid pid' int,
+  binds pid DInc5 st.(pc) ->
+  final_state register_counter_impl st pid' int st' ->
+  pid <> pid' ->
+  binds pid DInc5 st'.(pc).
+Proof.
+  inversion 2; intros; subst;
+  apply binds_remove in H;
+  simpl in *; try assumption;
+  apply notin_neq; auto.
+Qed. *)
+
+Section StrutureProperties.
+
+Variable A : Type.
+Implicit Types E F : env A.
+
+Lemma binds_neq_middle: forall F E x x1 v v1 v1',
+  binds x v (E ++ [(x1, v1)] ++ F) ->
+  x <> x1 ->
+  binds x v (E ++ [(x1, v1')] ++ F).
+Proof.
+  intros.
+  apply binds_concat_inv in H. intuition.
+  - eapply binds_concat_right; eauto.
+  - apply binds_concat_inv in H2. intuition.
+    -- unfold binds in H1. simpl in H1.
+      apply Nat.eqb_neq in H0.
+      rewrite H0 in H1. inversion H1.
+    -- eapply binds_concat_left; eauto.
+      eapply binds_push_neq; eauto.
+Qed.
+
+End StrutureProperties.
+
+
+Lemma step_preserves_binds_DInc5: forall st st' pid pid' int,
+  binds pid DInc5 st.(pc) ->
+  step register_counter_impl st pid' int st' ->
+  pid <> pid' ->
+  binds pid DInc5 st'.(pc).
+Proof.
+  inversion 2; intros; subst;
+  eapply binds_neq_middle; eauto.
+Qed.
+
+Lemma at_external_preserves_binds_DInc5: forall st st' pid pid' int,
+  binds pid DInc5 st.(pc) ->
+  at_external register_counter_impl st pid' int st' ->
+  binds pid DInc5 st'.(pc).
+Proof.
+  intros.
+  destruct (Nat.eq_dec pid pid').
+  - subst. inversion H0; subst; simpl in *.
+    -- apply binds_concat_inv in H. intuition.
+      --- eapply binds_concat_right; eauto.
+      --- unfold binds in H2. simpl in H2.
+        rewrite Nat.eqb_refl in H2. inversion H2.
+    -- apply binds_concat_inv in H. intuition.
+      --- eapply binds_concat_right; eauto.
+      --- unfold binds in H2. simpl in H2.
+        rewrite Nat.eqb_refl in H2. inversion H2.
+    -- apply binds_concat_inv in H. intuition.
+      --- eapply binds_concat_right; eauto.
+      --- unfold binds in H2. simpl in H2.
+        rewrite Nat.eqb_refl in H2. inversion H2.
+  - inversion H0; intros; subst;
+    eapply binds_neq_middle; eauto.
+Qed.
+
+Lemma after_external_preserves_binds_DInc5: forall st st' pid pid' int,
+  binds pid DInc5 st.(pc) ->
+  after_external register_counter_impl st pid' int st' ->
+  pid <> pid' ->
+  binds pid DInc5 st'.(pc).
+Proof.
+  inversion 2; intros; subst;
+  eapply binds_neq_middle; eauto.
+Qed.
+
+Lemma initial_preserves_binds_DInc5: forall st st' pid pid' int,
+  binds pid DInc5 st.(pc) ->
+  initial_state register_counter_impl st pid' int st' ->
+  (* pid <> pid' -> *)
+  binds pid DInc5 st'.(pc).
+Proof.
+  intros.
+  destruct (Nat.eq_dec pid pid').
+  - subst. inversion H0; subst; simpl in *;
+    apply binds_in in H; unfold "#" in H2; intuition.
+  - inversion H0; subst; simpl in *;
+    eapply binds_push_neq; eauto.
+Qed.
+
+Lemma final_preserves_binds_DInc5: forall st st' pid pid' int,
+  binds pid DInc5 st.(pc) ->
+  final_state register_counter_impl st pid' int st' ->
+  (* pid <> pid' -> *)
+  binds pid DInc5 st'.(pc).
+Proof.
+  intros.
+  destruct (Nat.eq_dec pid pid').
+  - subst. inversion H0; subst; simpl in *.
+    -- apply binds_concat_inv in H. intuition.
+      --- eapply binds_concat_right; eauto.
+      --- unfold binds in H2. simpl in H2.
+        rewrite Nat.eqb_refl in H2. inversion H2.
+    -- apply binds_concat_inv in H. intuition.
+      --- eapply binds_concat_right; eauto.
+      --- unfold binds in H2. simpl in H2.
+        rewrite Nat.eqb_refl in H2. inversion H2.
+  - inversion H0; intros; subst;
+    eapply binds_remove; eauto;
+    apply notin_neq; eauto.
+Qed.
+
+Lemma no_action_preserves_DInc5 : forall st st' pid acts in_acts,
+  binds pid DInc5 st.(pc) ->
+  gather_pid_internal_events in_acts pid = [] ->
+  gather_pid_external_events acts pid = [] ->
+  valid_execution_fragment register_counter_impl st st' acts in_acts ->
+  binds pid DInc5 st'.(pc).
+Proof.
+  intros. induction H2.
+  - subst. assumption.
+  - simpl in H0.
+    destruct (pid =? pid0)eqn:Heq.
+    -- inversion H0.
+    -- apply IHvalid_execution_fragment; auto.
+      eapply step_preserves_binds_DInc5; eauto.
+      eapply Nat.eqb_neq; eauto.
+  - simpl in H1.
+    destruct (pid =? pid0)eqn:Heq.
+    -- inversion H1.
+    -- apply IHvalid_execution_fragment; auto.
+      eapply at_external_preserves_binds_DInc5; eauto.
+  - simpl in H1.
+    destruct (pid =? pid0)eqn:Heq.
+    -- inversion H1.
+    -- apply IHvalid_execution_fragment; auto.
+      eapply after_external_preserves_binds_DInc5; eauto.
+      eapply Nat.eqb_neq; eauto.
+  - simpl in H1.
+    destruct (pid =? pid0)eqn:Heq.
+    -- inversion H1.
+    -- apply IHvalid_execution_fragment; auto.
+      eapply initial_preserves_binds_DInc5; eauto.
+  - simpl in H1.
+    destruct (pid =? pid0)eqn:Heq.
+    -- inversion H1.
+    -- apply IHvalid_execution_fragment; auto.
+      eapply final_preserves_binds_DInc5; eauto.
+Qed.
+
 (* 
   Potential problem: the mapping relation missed some details
 *)
@@ -253,7 +407,7 @@ Proof.
         subst. simpl in *.
 
         destruct H6 as [lst1 [lst2 [lst2st1 [lst2st2 [st1acts [st2acts [cs3 Htmp]]]]]]].
-        destruct Htmp as [Hbefore Hremain].
+        destruct Htmp as [st2in_acts [st1in_acts [Hbefore Hremain]]].
         inversion Hbefore; subst.
         inversion H11; subst.
         simpl in Hremain, Hbefore. intuition.
@@ -272,6 +426,9 @@ Proof.
         unfold binds. simpl. rewrite Nat.eqb_refl. reflexivity.
         apply ok_middle_inv in H5; intuition.
         inversion H6; subst. clear H6. simpl in *.
+        assert (Hst2: binds pid DInc5 st2.(pc)).
+        eapply no_action_preserves_DInc5; eauto.
+        eapply binds_concat_left; eauto.
         exists (mkCntState (requests s2) (responses s2) (S (value s2))).
 
         simpl.
